proof/extraction/XMSS_IMPL_PP.ec
@@ -40,6 +40,21 @@ module Mp(SC:SCall_t) = {
     return (out);
   }
 
+  proc __ull_to_bytes_4 (out:W8.t Array4.t, in_0:W64.t) : W8.t Array4.t = {
+    var aux: int;
+
+    var i:int;
+
+    aux <- (- 1);
+    i <- (4 - 1);
+    while (aux < i) {
+      out.[i] <- (truncateu8 in_0);
+      in_0 <- (in_0 `>>` (W8.of_int 8));
+      i <- i - 1;
+    }
+    return (out);
+  }
+
   proc __ull_to_bytes_2 (out:W8.t Array2.t, in_0:W64.t) : W8.t Array2.t = {
     var aux: int;
 
@@ -62,21 +77,6 @@ module Mp(SC:SCall_t) = {
 
     aux <- (- 1);
     i <- (32 - 1);
-    while (aux < i) {
-      out.[i] <- (truncateu8 in_0);
-      in_0 <- (in_0 `>>` (W8.of_int 8));
-      i <- i - 1;
-    }
-    return (out);
-  }
-
-  proc __ull_to_bytes_4 (out:W8.t Array4.t, in_0:W64.t) : W8.t Array4.t = {
-    var aux: int;
-
-    var i:int;
-
-    aux <- (- 1);
-    i <- (4 - 1);
     while (aux < i) {
       out.[i] <- (truncateu8 in_0);
       in_0 <- (in_0 `>>` (W8.of_int 8));
@@ -249,8 +249,8 @@ module Mp(SC:SCall_t) = {
     return (out);
   }
 
-  proc __memcpy_u8u8_64_32 (out:W8.t Array64.t, in_0:W8.t Array32.t) : 
-  W8.t Array64.t = {
+  proc __memcpy_u8u8_32_32 (out:W8.t Array32.t, in_0:W8.t Array32.t) : 
+  W8.t Array32.t = {
 
     var i:W64.t;
 
@@ -263,8 +263,8 @@ module Mp(SC:SCall_t) = {
     return (out);
   }
 
-  proc __memcpy_u8u8_32_32 (out:W8.t Array32.t, in_0:W8.t Array32.t) : 
-  W8.t Array32.t = {
+  proc __memcpy_u8u8_64_32 (out:W8.t Array64.t, in_0:W8.t Array32.t) : 
+  W8.t Array64.t = {
 
     var i:W64.t;
 
@@ -284,6 +284,13 @@ module Mp(SC:SCall_t) = {
     return (out);
   }
 
+  proc _memcpy_u8u8_32_32 (out:W8.t Array32.t, in_0:W8.t Array32.t) : 
+  W8.t Array32.t = {
+
+    out <@ __memcpy_u8u8_32_32 (out, in_0);
+    return (out);
+  }
+
   proc _memcpy_u8u8_64_32 (out:W8.t Array64.t, in_0:W8.t Array32.t) : 
   W8.t Array64.t = {
 
@@ -291,10 +298,13 @@ module Mp(SC:SCall_t) = {
     return (out);
   }
 
-  proc _memcpy_u8u8_32_32 (out:W8.t Array32.t, in_0:W8.t Array32.t) : 
+  proc _x_memcpy_u8u8_32_32 (out:W8.t Array32.t, in_0:W8.t Array32.t) : 
   W8.t Array32.t = {
 
-    out <@ __memcpy_u8u8_32_32 (out, in_0);
+    out <- out;
+    in_0 <- in_0;
+    out <@ _memcpy_u8u8_32_32 (out, in_0);
+    out <- out;
     return (out);
   }
 
@@ -314,16 +324,6 @@ module Mp(SC:SCall_t) = {
     out <- out;
     in_0 <- in_0;
     out <@ _memcpy_u8u8_64_32 (out, in_0);
-    out <- out;
-    return (out);
-  }
-
-  proc _x_memcpy_u8u8_32_32 (out:W8.t Array32.t, in_0:W8.t Array32.t) : 
-  W8.t Array32.t = {
-
-    out <- out;
-    in_0 <- in_0;
-    out <@ _memcpy_u8u8_32_32 (out, in_0);
     out <- out;
     return (out);
   }
@@ -2278,6 +2278,22 @@ module Mp(SC:SCall_t) = {
 
     res_0 <@ __xmss_sign_open (pk, m_ptr, mlen_ptr, sm_ptr, smlen);
     return (res_0);
+  }
+
+  proc __memswap_32 (a:W8.t Array32.t, b:W8.t Array32.t, t:W8.t Array32.t) : 
+  W8.t Array32.t * W8.t Array32.t * W8.t Array32.t = {
+
+    t <@ _x_memcpy_u8u8_32_32 (t, a);
+    a <@ _x_memcpy_u8u8_32_32 (a, b);
+    b <@ _x_memcpy_u8u8_32_32 (b, t);
+    return (a, b, t);
+  }
+
+  proc memswap (a:W8.t Array32.t, b:W8.t Array32.t, t:W8.t Array32.t) : 
+  W8.t Array32.t * W8.t Array32.t * W8.t Array32.t = {
+
+    (a, b, t) <@ __memswap_32 (a, b, t);
+    return (a, b, t);
   }
 }.
 
